string_of_term and fix check_eq/check_leq w.r.t. constraints

theories/Checker.v
@@ -173,12 +173,12 @@ Definition isConstruct c :=
 
 Inductive conv_pb :=
 | Conv
-| Cumul (φ : uGraph.t).
+| Cumul.
 
 Section Conversion.
 
   Context (flags : RedFlags.t).
-  Context (Σ : global_declarations).
+  Context (Σ : global_context).
 
   Definition nodelta_flags := RedFlags.mk true true true false true true.
 
@@ -186,14 +186,14 @@ Section Conversion.
     unf <- unfold_fix mfix idx ;;
     let '(arg, fn) := unf in
     c <- nth_error l arg ;;
-    cred <- reduce_stack RedFlags.default Σ Γ n c [] ;;
+    cred <- reduce_stack RedFlags.default (fst Σ) Γ n c [] ;;
     let '(cred, _) := cred in
-    if eq_term cred c || negb (isConstruct cred) then None
+    if eq_term (snd Σ) cred c || negb (isConstruct cred) then None
     else Some fn.
 
   Definition unfold_one_case n Γ c :=
-    cred <- reduce_stack_term RedFlags.default Σ Γ n c ;;
-    if eq_term cred c then None
+    cred <- reduce_stack_term RedFlags.default (fst Σ) Γ n c ;;
+    if eq_term (snd Σ) cred c then None
     else Some cred.
 
   Definition reducible_head n Γ c l :=
@@ -205,18 +205,20 @@ Section Conversion.
       | Some c' => Some (tCase ind' p' c' brs)
       end
     | tConst c _ => (* TODO Universes *)
-      match lookup_env Σ c with
+      match lookup_env (fst Σ) c with
       | Some (ConstantDecl _ {| cst_body := Some body |}) => Some body
       | _ => None
       end
     | _ => None
     end.
 
+  Definition lookup_env c := lookup_env (fst Σ) c.
+
   Fixpoint isconv (n : nat) (leq : conv_pb) (Γ : context)
            (t1 : term) (l1 : list term) (t2 : term) (l2 : list term) {struct n} : option bool :=
     match n with 0 => None | S n =>
-    red1 <- reduce_stack nodelta_flags Σ Γ n t1 l1 ;;
-    red2 <- reduce_stack nodelta_flags Σ Γ n t2 l2 ;;
+    red1 <- reduce_stack nodelta_flags (fst Σ) Γ n t1 l1 ;;
+    red2 <- reduce_stack nodelta_flags (fst Σ) Γ n t2 l2 ;;
     let '(t1,l1) := red1 in
     let '(t2,l2) := red1 in
     isconv_prog n leq Γ t1 l1 t2 l2
@@ -234,16 +236,16 @@ Section Conversion.
     let fallback (x : unit) :=
       match reducible_head n Γ t1 l1 with
       | Some t1 =>
-        redt <- reduce_stack nodelta_flags Σ Γ n t1 l1 ;;
+        redt <- reduce_stack nodelta_flags (fst Σ) Γ n t1 l1 ;;
         let '(t1, l1) := redt in
         isconv_prog n leq Γ t1 l1 t2 l2
       | None =>
         match reducible_head n Γ t2 l2 with
         | Some t2 =>
-          redt <- reduce_stack nodelta_flags Σ Γ n t2 l2 ;;
+          redt <- reduce_stack nodelta_flags (fst Σ) Γ n t2 l2 ;;
           let '(t2, l2) := redt in
           isconv_prog n leq Γ t1 l1 t2 l2
-        | None => on_cond (match leq with Conv => eq_term t1 t2 | Cumul φ => leq_term φ t1 t2 end)
+        | None => on_cond (match leq with Conv => eq_term (snd Σ) t1 t2 | Cumul => leq_term (snd Σ) t1 t2 end)
         end
       end
     in
@@ -258,17 +260,17 @@ Section Conversion.
         b <- isconv_stacks l1 l2 ;;
         if b then ret true (* FO optim *)
         else
-          match lookup_env Σ c with (* Unfold both bodies at once *)
+          match lookup_env c with (* Unfold both bodies at once *)
           | Some (ConstantDecl _ {| cst_body := Some body |}) =>
             isconv n leq Γ body l1 body l2
           | _ => ret false
           end
       else
-        match lookup_env Σ c' with
+        match lookup_env c' with
         | Some (ConstantDecl _ {| cst_body := Some body |}) =>
           isconv n leq Γ t1 l1 body l2
         | _ =>
-          match lookup_env Σ c with
+          match lookup_env c with
           | Some (ConstantDecl _ {| cst_body := Some body |}) =>
             isconv n leq Γ body l1 t2 l2
           | _ => ret false
@@ -289,30 +291,30 @@ Section Conversion.
 
     | tCase (ind, par) p c brs,
       tCase (ind',par') p' c' brs' => (* Hnf did not reduce, maybe delta needed in c *)
-      if eq_term p p' && eq_term c c' && forallb2 (fun '(a, b) '(a', b') => eq_term b b') brs brs' then
+      if eq_term (snd Σ) p p' && eq_term (snd Σ) c c' && forallb2 (fun '(a, b) '(a', b') => eq_term (snd Σ) b b') brs brs' then
         ret true
       else
-        cred <- reduce_stack_term RedFlags.default Σ Γ n c ;;
-        c'red <- reduce_stack_term RedFlags.default Σ Γ n c' ;;
-        if eq_term cred c && eq_term c'red c' then ret false
+        cred <- reduce_stack_term RedFlags.default (fst Σ) Γ n c ;;
+        c'red <- reduce_stack_term RedFlags.default (fst Σ) Γ n c' ;;
+        if eq_term (snd Σ) cred c && eq_term (snd Σ) c'red c' then ret false
         else
           isconv n leq Γ (tCase (ind, par) p cred brs) l1 (tCase (ind, par) p c'red brs') l2
 
-    | tProj p c, tProj p' c' => on_cond (eq_projection p p' && eq_term c c')
+    | tProj p c, tProj p' c' => on_cond (eq_projection p p' && eq_term (snd Σ) c c')
 
     | tFix mfix idx, tFix mfix' idx' =>
       (* Hnf did not reduce, maybe delta needed *)
-      if eq_term t1 t2 && match isconv_stacks l1 l2 with Some b => b | None => false end then ret true
+      if eq_term (snd Σ) t1 t2 && match isconv_stacks l1 l2 with Some b => b | None => false end then ret true
       else
         match unfold_one_fix n Γ mfix idx l1 with
         | Some t1 =>
-          redt <- reduce_stack nodelta_flags Σ Γ n t1 l1 ;;
+          redt <- reduce_stack nodelta_flags (fst Σ) Γ n t1 l1 ;;
           let '(t1, l1) := redt in
           isconv_prog n leq Γ t1 l1 t2 l2
         | None =>
           match unfold_one_fix n Γ mfix' idx' l2 with
           | Some t2 =>
-            redt <- reduce_stack nodelta_flags Σ Γ n t2 l2 ;;
+            redt <- reduce_stack nodelta_flags (fst Σ) Γ n t2 l2 ;;
             let '(t2, l2) := redt in
             isconv_prog n leq Γ t1 l1 t2 l2
           | None => ret false
@@ -320,7 +322,7 @@ Section Conversion.
         end
 
     | tCoFix mfix idx, tCoFix mfix' idx' =>
-      on_cond (eq_term t1 t2)
+      on_cond (eq_term (snd Σ) t1 t2)
 
     | _, _ => fallback ()
     end
@@ -362,6 +364,65 @@ Inductive type_error :=
 
 Definition string_of_nat (n : nat) := Template.utils.string_of_int n.
 
+Definition string_of_list_aux {A} (f : A -> string) (l : list A) : string :=
+  let fix aux l :=
+      match l with
+      | nil => ""
+      | cons a nil => f a
+      | cons a l => f a ++ "," ++ aux l
+      end
+  in aux l.
+
+Definition string_of_list {A} (f : A -> string) (l : list A) : string :=
+  "[" ++ string_of_list_aux f l ++ "]".
+
+Definition string_of_level (l : Level.t) : string :=
+  match l with
+  | Level.lProp => "Prop"
+  | Level.lSet => "Set"
+  | Level.Level s => s
+  | Level.Var n => "Var" ++ string_of_nat n
+  end.
+
+Definition string_of_level_expr (l : Level.t * bool) : string :=
+  let '(l, b) := l in
+  string_of_level l ++ (if b then "+1" else "").
+
+Definition string_of_sort (u : universe) :=
+  string_of_list string_of_level_expr u.
+Definition string_of_name (na : name) :=
+  match na with
+  | nAnon => "Anonymous"
+  | nNamed n => n
+  end.
+Definition string_of_universe_instance u :=
+  string_of_list string_of_level u.
+
+Fixpoint string_of_term (t : term) :=
+  match t with
+  | tRel n => "Rel(" ++ string_of_nat n ++ ")"
+  | tVar n => "Var(" ++ n ++ ")"
+  | tMeta n => "Meta(" ++ string_of_nat n ++ ")"
+  | tEvar ev args => "Evar(" ++ string_of_nat ev ++ "[]" (* TODO *)  ++ ")"
+  | tSort s => "Sort(" ++ string_of_sort s ++ ")"
+  | tCast c k t => "Cast(" ++ string_of_term c ++ (* TODO *) "," ++ string_of_term t ++ ")"
+  | tProd na b t => "Prod(" ++ string_of_name na ++ "," ++ string_of_term b ++ "," ++ string_of_term t ++ ")"
+  | tLambda na b t => "Lambda(" ++ string_of_name na ++ "," ++ string_of_term b ++ "," ++ string_of_term t ++ ")"
+  | tLetIn na b t' t => "LetIn(" ++ string_of_name na ++ "," ++ string_of_term b ++ "," ++ string_of_term t' ++ "," ++ string_of_term t ++ ")"
+  | tApp f l => "App(" ++ string_of_term f ++ "," ++ string_of_list string_of_term l ++ ")"
+  | tConst c u => "Const(" ++ c ++ "," ++ string_of_universe_instance u ++ ")"
+  | tInd (mkInd c i) u => "Ind(" ++ c ++ "," ++ string_of_int i ++ "," ++ string_of_universe_instance u ++ ")"
+  | tConstruct (mkInd c i) n u => "Construct(" ++ c ++ "," ++ string_of_int i ++ "," ++
+                                               string_of_int n ++ "," ++
+                                               string_of_universe_instance u ++ ")"
+  | tCase (ind, i) t p brs =>
+    "Case(" ++ string_of_term t ++ "," ++ string_of_term p ++ "," ++
+            string_of_list (fun b => string_of_term (snd b)) brs ++ ")"
+  | tProj p c =>
+    "Proj(" ++ "TODO" ++ "," ++ string_of_term c ++ ")"
+  | _ => "TODO string_of_term"
+  end.
+
 Definition string_of_type_error (e : type_error) : string :=
   match e with
   | UnboundRel n => "Unboound rel " ++ string_of_nat n
@@ -371,7 +432,9 @@ Definition string_of_type_error (e : type_error) : string :=
   | UndeclaredConstant c => "Undeclared constant " ++ c
   | UndeclaredInductive c => "Undeclared inductive " ++ (inductive_mind c)
   | UndeclaredConstructor c i => "Undeclared inductive " ++ (inductive_mind c)
-  | NotConvertible Γ t u t' u' => "Terms are not convertible"
+  | NotConvertible Γ t u t' u' => "Terms are not convertible: " ++
+      string_of_term t ++ " " ++ string_of_term u ++ " after reduction: " ++
+      string_of_term t' ++ " " ++ string_of_term u'
   | NotASort t => "Not a sort"
   | NotAProduct t t' => "Not a product"
   | NotAnInductive t => "Not an inductive"
@@ -412,14 +475,14 @@ Definition check_conv_gen {F:Fuel} conv_pb Σ Γ t u :=
   | None => raise (NotEnoughFuel fuel)
   end.
 
-Definition check_conv_leq {F:Fuel} φ := check_conv_gen (Cumul φ).
+Definition check_conv_leq {F:Fuel} := check_conv_gen Cumul.
 Definition check_conv {F:Fuel} := check_conv_gen Conv.
 
 Conjecture conv_spec : forall {F:Fuel} Σ Γ t u,
-    Σ ;;; Γ |- t = u <-> check_conv (fst Σ) Γ t u = Checked ().
+    Σ ;;; Γ |- t = u <-> check_conv Σ Γ t u = Checked ().
 
 Conjecture cumul_spec : forall {F:Fuel} Σ Γ t u,
-    Σ ;;; Γ |- t <= u <-> check_conv_leq (snd Σ) (fst Σ) Γ t u = Checked ().
+    Σ ;;; Γ |- t <= u <-> check_conv_leq Σ Γ t u = Checked ().
 
 Conjecture reduce_cumul : forall Σ Γ n t, Σ ;;; Γ |- try_reduce (fst Σ) Γ n t <= t.
 
@@ -467,9 +530,9 @@ Section Typecheck2.
   Context (Σ : global_context).
 
   Definition convert_leq Γ (t u : term) : typing_result unit :=
-    if eq_term t u then ret ()
+    if eq_term (snd Σ) t u then ret ()
     else
-      match isconv (fst Σ) fuel (Cumul (snd Σ)) Γ t [] u [] with
+      match isconv Σ fuel Cumul Γ t [] u [] with
       | Some b =>
         if b then ret ()
         else raise (NotConvertible Γ t u t u)
@@ -512,7 +575,7 @@ Section Typecheck2.
     end.
 
   Definition lookup_constant_type cst u :=
-    match lookup_env (fst Σ) cst with
+    match lookup_env Σ cst with
     | Some (ConstantDecl _ {| cst_type := ty; cst_universes := uctx |}) =>
       let cstrs := polymorphic_constraints uctx in
       ret (subst_instance_constr u ty, subst_instance_cstrs u cstrs)
@@ -520,7 +583,7 @@ Section Typecheck2.
     end.
 
   Definition lookup_ind_type ind i (u : list Level.t) (* TODO Universes *) :=
-    match lookup_env (fst Σ) ind with
+    match lookup_env Σ ind with
     | Some (InductiveDecl _ {| ind_bodies := l; ind_universes := uctx |}) =>
       match nth_error l i with
       | Some body =>
@@ -532,7 +595,7 @@ Section Typecheck2.
     end.
 
   Definition lookup_constructor_type ind i k u :=
-    match lookup_env (fst Σ) ind with
+    match lookup_env Σ ind with
     | Some (InductiveDecl _ {| ind_bodies := l ; ind_universes := uctx |}) =>
       match nth_error l i with
       | Some body =>
@@ -679,9 +742,10 @@ Section Typecheck2.
         reduce_to_ind (fst Σ) Γ t = Checked (i, u, args') /\
         cumul Σ Γ (mkApps (tInd i u) args') (mkApps (tInd i u) args).
 
-  Lemma lookup_env_id {id decl} : lookup_env (fst Σ) id = Some decl -> id = global_decl_ident decl.
+  Lemma lookup_env_id {id decl} : lookup_env Σ id = Some decl -> id = global_decl_ident decl.
   Proof.
     destruct Σ.
+    unfold lookup_env.
     induction g; simpl; intros; try discriminate; trivial.
     revert H. destruct (ident_eq_spec id (global_decl_ident a)). now intros [= ->].
     apply IHg.
@@ -691,7 +755,8 @@ Section Typecheck2.
     lookup_constant_type cst u =
     Checked (subst_instance_constr u decl.(cst_type), subst_instance_cstrs u (polymorphic_constraints decl.(cst_universes))).
   Proof.
-    unfold lookup_constant_type. red in isdecl. rewrite isdecl. destruct decl. reflexivity.
+    unfold lookup_constant_type, lookup_env.
+    red in isdecl. rewrite isdecl. destruct decl. reflexivity.
   Qed.
   
   Lemma lookup_constant_type_is_declared cst u T :
@@ -699,8 +764,8 @@ Section Typecheck2.
     { decl | declared_constant (fst Σ) cst decl /\
              subst_instance_constr u decl.(cst_type) = fst T }.
   Proof.
-    unfold lookup_constant_type, declared_constant.
-    destruct lookup_env eqn:Hlook; try discriminate.
+    unfold lookup_constant_type, lookup_env, declared_constant.
+    destruct Typing.lookup_env eqn:Hlook; try discriminate.
     destruct g eqn:Hg; intros; try discriminate. destruct c.
     injection H as eq. subst T. rewrite (lookup_env_id Hlook). simpl.
     eexists. split; eauto.
